src/lowparse/LowParse.SLow.Bytes.fst
@@ -1,4 +1,5 @@
 module LowParse.SLow.Bytes
+open FStar.Error // for Correct, Error
 include LowParse.Spec.Bytes
 include LowParse.SLow.VLData
 
@@ -45,8 +46,8 @@ inline_for_extraction
 let parse32_all_bytes
   : parser32 parse_all_bytes
 = fun (input: B32.bytes) ->
-    let res = Some (input, B32.len input) in
-    (res <: (res: option (bytes32 * U32.t) { parser32_correct parse_all_bytes input res } ))
+    let res = Correct (input, B32.len input) in
+    (res <: (res: result (bytes32 * U32.t) { parser32_correct parse_all_bytes input res } ))
 
 inline_for_extraction
 let serialize32_all_bytes
